src/Rewriter/Util/plugins/RewriterBuildRegistryImports.v
@@ -1,4 +1,5 @@
 Require Export Rewriter.Language.Pre.
+Require Import Rewriter.Language.PreLemmas.
 Require Export Rewriter.Language.IdentifiersBasicGenerate.
 Require Export Rewriter.Rewriter.ProofsCommon.
 Require Export Rewriter.Rewriter.AllTactics.
@@ -6,5 +7,6 @@ Require Import Rewriter.Util.plugins.StrategyTactic.
 Export IdentifiersBasicGenerate.Compilers.
 Export ProofsCommon.Compilers.
 Export AllTactics.Compilers.
+Export PreLemmas.Instances.
 
 Ltac Pre.set_strategy_expand name ::= strategy -1000 [name].
